Get rid of mlifyable_in typeclass

io/ho_examples/Callback.Level1.fst
@@ -54,32 +54,29 @@ assume val pp_pre : trace -> Type0
 assume val pp_post : trace -> maybe pp_out -> trace -> Type0
 type pp = ctx -> IIO (maybe pp_out) pp_pre pp_post
 
+
 assume val pp_cb_pre_checkable : checkable2 pp_cb_pre
 
 assume val pp_monitorable_hist : monitorable_hist pp_cb_pre pp_cb_post pi
 
-let pp_cb_mlifyable_in : mlifyable_in_arr1 pp_cb_in pp_cb_out pp_cb_pre pp_cb_post pi = {
-  cmlifyable1 = 
-    mlifyable_iiowp_trivialize_weaken_post
-      pp_cb_in #pp_cb_in_importable
-      pp_cb_out #pp_cb_out_exportable
-      pp_cb_pre #pp_cb_pre_checkable
-      pp_cb_post
-      pi #pp_monitorable_hist;
-  ca1 = pp_cb_in_importable;
-}
+let pp_cb_mlifyable : mlifyable pp_cb pi =
+  mlifyable_iiowp_trivialize_weaken_post
+    pp_cb_in #pp_cb_in_importable
+    pp_cb_out #pp_cb_out_exportable
+    pp_cb_pre #pp_cb_pre_checkable
+    pp_cb_post
+    pi #pp_monitorable_hist
 
-assume val ctx_post_monitorable : checkable_hist_post #pp_cb_mlifyable_in.cmlifyable1.matype (fun x -> ctx_pre) (fun x -> ctx_post) pi
+assume val ctx_post_monitorable : checkable_hist_post #pp_cb_mlifyable.matype (fun x -> ctx_pre) (fun x -> ctx_post) pi
 
 let ctx_instrumentable : instrumentable ctx pi =
   instrumentable_HO_arr1_out_importable
-    pp_cb_in pp_cb_out pp_cb_pre pp_cb_post
+    pp_cb
     ctx_out ctx_pre ctx_post
     pi
     #ctx_out_importable
-    #pp_cb_mlifyable_in
+    #pp_cb_mlifyable
     #ctx_post_monitorable
-
 
 assume val pp_pre_checkable : checkable pp_pre
   
